Examples/SystemFWithNat/Term.lean
@@ -4,6 +4,16 @@ open LeanSubst
 
 namespace SystemFWithNat
 
+@[simp]
+theorem Subst.test {T n} : n :: Ren.add T (n + 1) = Ren.add T n := by
+  induction n; simp
+  simp [Ren.add, Ren.cons] at *
+  funext; case _ i =>
+  cases i <;> simp; omega
+
+@[simp]
+theorem Subst.test2 {T V} [RenMap T V] (r : RenVec V) : (Subst.id T)⟨r,⟩ = Subst.id T := sorry
+
 inductive Ty where
 | var : Nat -> Ty
 | arrow : Ty -> Ty -> Ty
@@ -55,6 +65,9 @@ def Ty.rmap (r : RenVec [Ty]) : Ty -> Ty
 instance : RenMap Ty [Ty] where
   rmap := Ty.rmap
 
+@[reducible, simp]
+instance instRenMapAll_Ty : RenMapAll [Ty] := .cons .nil
+
 @[simp]
 theorem Ty.rmap_var {x} {r : RenVec [Ty]} : (var x)⟨r,⟩ = .var ((r.get Ty 0).act x) := by
   simp [RenMap.rmap]
@@ -92,11 +105,10 @@ def Ty.smap (σ : SubstVec [Ty]) : Ty -> Ty
 | arrow t1 t2 => arrow (t1.smap σ) (t2.smap σ)
 | all t => all $ t.smap $ σ.lift [1]
 
-instance instSubstMap_Ty_Ty : SubstMap Ty [Ty] where
+instance : SubstMap Ty [Ty] where
   smap := Ty.smap
 
-instance : SubstMapAll [Ty] :=
-  .cons instSubstMap_Ty_Ty sorry .nil
+instance instSubstMapAll_Ty : SubstMapAll [Ty] := .cons .nil
 
 @[simp]
 theorem Ty.smap_var {x} {σ : SubstVec [Ty]} : (var x)[σ,] = (σ.get Ty 0).act x := by
@@ -129,10 +141,10 @@ instance : SubstMapStable Ty [Ty] where
   apply_stable := by sorry
 
 instance : SubstMapRenComposeLeft Ty [Ty] where
-  apply_ren_compose_left := by sorry
+  apply_ren_compose_left := by subst_solve_compose
 
 instance : SubstMapRenComposeRight Ty [Ty] where
-  apply_ren_compose_right := by sorry
+  apply_ren_compose_right := by subst_solve_compose
 
 instance : SubstMapCompose Ty [Ty] where
   apply_compose := by sorry
@@ -176,46 +188,126 @@ def Term.rmap (r : RenVec [Term, Ty]) : Term -> Term
 instance : RenMap Term [Term, Ty] where
   rmap := Term.rmap
 
-instance : RenMap Term [Term] where
-  rmap r := Term.rmap (r.1, Ren.id Ty, .unit)
+@[simp]
+theorem Term.rmap_term_ty_var {x} {r : RenVec [Term, Ty]} : (var x)⟨r,⟩ = var ((r.get Term 0).act x) := by
+  simp [RenMap.rmap]
+
+@[simp]
+theorem Term.rmap_term_ty_app {t1 t2} {r : RenVec [Term, Ty]} : (app t1 t2)⟨r,⟩ = app t1⟨r,⟩ t2⟨r,⟩ := by
+  simp [RenMap.rmap]
+
+@[simp]
+theorem Term.rmap_term_ty_lam {A t} {r : RenVec [Term, Ty]}
+  : (lam A t)⟨r,⟩ = lam A⟨r.get Ty 1⟩ t⟨r.lift [1, 0],⟩
+:= by simp [RenMap.rmap]
+
+@[simp]
+theorem Term.rmap_term_ty_tapp {t1 t2} {r : RenVec [Term, Ty]}
+  : (tapp t1 t2)⟨r,⟩ = tapp t1⟨r,⟩ t2⟨r.get Ty 1⟩
+:= by simp [RenMap.rmap]
+
+@[simp]
+theorem Term.rmap_term_ty_tlam {t} {r : RenVec [Term, Ty]} : (tlam t)⟨r,⟩ = tlam t⟨r.lift [0, 1],⟩ := by
+  simp [RenMap.rmap]
+
+@[simp]
+theorem Term.rmap_term_ty_zero {r : RenVec [Term, Ty]} : zero⟨r,⟩ = zero := by
+  simp [RenMap.rmap]
+
+@[simp]
+theorem Term.rmap_term_ty_succ {t} {r : RenVec [Term, Ty]} : (succ t)⟨r,⟩ = succ t⟨r,⟩ := by
+  simp [RenMap.rmap]
+
+@[simp]
+theorem Term.rmap_term_ty_nrec {m z s n} {r : RenVec [Term, Ty]}
+  : (nrec m z s n)⟨r,⟩ = nrec m⟨r.get Ty 1⟩ z⟨r,⟩ s⟨r.lift [2, 0],⟩ n⟨r,⟩
+:= by simp [RenMap.rmap]
 
 instance : RenMap Term [Ty] where
   rmap r := Term.rmap (Ren.id Term, r.1, .unit)
 
 @[simp]
-theorem Term.rmap_var {x} {r : RenVec [Term, Ty]} : (var x)⟨r,⟩ = var ((r.get Term 0).act x) := by
+theorem Term.rmap_ty_var {x} {r : RenVec [Ty]} : (var x)⟨r,⟩ = var x := by
   simp [RenMap.rmap]
 
 @[simp]
-theorem Term.rmap_app {t1 t2} {r : RenVec [Term, Ty]} : (app t1 t2)⟨r,⟩ = app t1⟨r,⟩ t2⟨r,⟩ := by
+theorem Term.rmap_ty_app {t1 t2} {r : RenVec [Ty]} : (app t1 t2)⟨r,⟩ = app t1⟨r,⟩ t2⟨r,⟩ := by
   simp [RenMap.rmap]
 
 @[simp]
-theorem Term.rmap_lam {A t} {r : RenVec [Term, Ty]}
-  : (lam A t)⟨r,⟩ = lam A⟨r.get Ty 1⟩ t⟨r.lift [1, 0],⟩
-:= by simp [RenMap.rmap]
+theorem Term.rmap_ty_lam {A t} {r : RenVec [Ty]}
+  : (lam A t)⟨r,⟩ = lam A⟨r.get Ty 0⟩ t⟨r,⟩
+:= by simp [RenMap.rmap]; try grind
 
 @[simp]
-theorem Term.rmap_tapp {t1 t2} {r : RenVec [Term, Ty]}
-  : (tapp t1 t2)⟨r,⟩ = tapp t1⟨r,⟩ t2⟨r.get Ty 1⟩
-:= by simp [RenMap.rmap]
+theorem Term.rmap_ty_tapp {t1 t2} {r : RenVec [Ty]}
+  : (tapp t1 t2)⟨r,⟩ = tapp t1⟨r,⟩ t2⟨r.get Ty 0⟩
+:= by simp [RenMap.rmap]; try grind
 
 @[simp]
-theorem Term.rmap_tlam {t} {r : RenVec [Term, Ty]} : (tlam t)⟨r,⟩ = tlam t⟨r.lift [0, 1],⟩ := by
+theorem Term.rmap_ty_tlam {t} {r : RenVec [Ty]} : (tlam t)⟨r,⟩ = tlam t⟨r.lift [1],⟩ := by
+  simp +instances [RenMap.rmap]
+  rcases r with ⟨r, u⟩; cases u -- TODO(FIX)
+  simp
+
+@[simp]
+theorem Term.rmap_ty_zero {r : RenVec [Ty]} : zero⟨r,⟩ = zero := by
   simp [RenMap.rmap]
 
 @[simp]
-theorem Term.rmap_zero {r : RenVec [Term, Ty]} : zero⟨r,⟩ = zero := by
+theorem Term.rmap_ty_succ {t} {r : RenVec [Ty]} : (succ t)⟨r,⟩ = succ t⟨r,⟩ := by
   simp [RenMap.rmap]
 
 @[simp]
-theorem Term.rmap_succ {t} {r : RenVec [Term, Ty]} : (succ t)⟨r,⟩ = succ t⟨r,⟩ := by
+theorem Term.rmap_ty_nrec {m z s n} {r : RenVec [Ty]}
+  : (nrec m z s n)⟨r,⟩ = nrec m⟨r.get Ty 0⟩ z⟨r,⟩ s⟨r,⟩ n⟨r,⟩
+:= by simp [RenMap.rmap]; grind
+
+instance : RenMap Term [Term] where
+  rmap r := Term.rmap (r.1, Ren.id Ty, .unit)
+
+@[simp]
+theorem Term.rmap_term_var {x} {r : RenVec [Term]} : (var x)⟨r,⟩ = var ((r.get Term 0).act x) := by
+  simp [RenMap.rmap]
+  rcases r with ⟨r, u⟩; cases u -- TODO(FIX)
+  simp
+
+@[simp]
+theorem Term.rmap_term_app {t1 t2} {r : RenVec [Term]} : (app t1 t2)⟨r,⟩ = app t1⟨r,⟩ t2⟨r,⟩ := by
   simp [RenMap.rmap]
 
 @[simp]
-theorem Term.rmap_nrec {m z s n} {r : RenVec [Term, Ty]}
-  : (nrec m z s n)⟨r,⟩ = nrec m⟨r.get Ty 1⟩ z⟨r,⟩ s⟨r.lift [2, 0],⟩ n⟨r,⟩
-:= by simp [RenMap.rmap]
+theorem Term.rmap_term_lam {A t} {r : RenVec [Term]}
+  : (lam A t)⟨r,⟩ = lam A t⟨r.lift [1],⟩
+:= by sorry
+
+@[simp]
+theorem Term.rmap_term_tapp {t1 t2} {r : RenVec [Term]}
+  : (tapp t1 t2)⟨r,⟩ = tapp t1⟨r,⟩ t2
+:= by sorry
+
+@[simp]
+theorem Term.rmap_term_tlam {t} {r : RenVec [Term]} : (tlam t)⟨r,⟩ = tlam t⟨r,⟩ := by
+  simp [RenMap.rmap]
+
+@[simp]
+theorem Term.rmap_term_zero {r : RenVec [Term]} : zero⟨r,⟩ = zero := by
+  simp [RenMap.rmap]
+
+@[simp]
+theorem Term.rmap_term_succ {t} {r : RenVec [Term]} : (succ t)⟨r,⟩ = succ t⟨r,⟩ := by
+  simp [RenMap.rmap]
+
+@[simp]
+theorem Term.rmap_term_nrec {m z s n} {r : RenVec [Term]}
+  : (nrec m z s n)⟨r,⟩ = nrec m z⟨r,⟩ s⟨r.lift [2],⟩ n⟨r,⟩
+:= by sorry
+
+@[reducible, simp]
+instance instRenMapAll_Term : RenMapAll [Term] := .cons .nil
+
+@[reducible, simp]
+instance instRenMapAll_Term_Ty : RenMapAll [Term, Ty] := .cons instRenMapAll_Ty
 
 -- @[simp]
 -- theorem Term.from_action_rmap {t : Action Term} {r : RenVec [Term, Ty]}
@@ -225,27 +317,20 @@ theorem Term.rmap_nrec {m z s n} {r : RenVec [Term, Ty]}
 --   cases u; case _ =>
 --   cases t <;> simp [Term.from_action, RenVec.get]
 
-@[simp]
-theorem Subst.test {T n} : n :: Ren.add T (n + 1) = Ren.add T n := by
-  induction n; simp
-  simp [Ren.add, Ren.cons] at *
-  funext; case _ i =>
-  cases i <;> simp; omega
-
 instance : RenMapId Term [Term, Ty] where
   apply_id := by subst_solve_id
 
 instance : RenMapCompose Term [Term, Ty] where
-  apply_compose := by subst_solve_compose
+  apply_compose := by sorry
 
 instance : RenMapId Term [Term] where
-  apply_id := sorry
+  apply_id := by subst_solve_id
 
 instance : RenMapCompose Term [Term] where
   apply_compose := by sorry
 
 instance : RenMapId Term [Ty] where
-  apply_id := sorry
+  apply_id := by subst_solve_id
 
 instance : RenMapCompose Term [Ty] where
   apply_compose := by sorry
@@ -266,58 +351,126 @@ instance : SubstMap Term [Term, Ty] where
   smap := Term.smap
 
 @[simp]
-instance instSubstMap_Term_Term : SubstMap Term [Term] where
-  smap σ := Term.smap (σ.get Term 0, Subst.id Ty, .unit)
-
-@[simp]
-instance instSubstMap_Term_Ty : SubstMap Term [Ty] where
-  smap σ := Term.smap (Subst.id Term, σ.get Ty 0, .unit)
-
-instance : SubstMapAll [Term] :=
-  .cons instSubstMap_Term_Term sorry .nil
-
-instance : SubstMapAll [Term, Ty] :=
-  .cons instSubstMap_Term_Term instSubstMap_Term_Ty
-    $ .cons instSubstMap_Ty_Ty sorry .nil
-
-@[simp]
-theorem Term.smap_var {x} {σ : SubstVec [Term, Ty]} : (var x)[σ,] = (σ.get Term 0).act x := by
+theorem Term.smap_term_ty_var {x} {σ : SubstVec [Term, Ty]} : (var x)[σ,] = (σ.get Term 0).act x := by
   simp [SubstMap.smap]
 
 @[simp]
-theorem Term.smap_app {t1 t2} {σ : SubstVec [Term, Ty]} : (app t1 t2)[σ,] = app t1[σ,] t2[σ,] := by
+theorem Term.smap_term_ty_app {t1 t2} {σ : SubstVec [Term, Ty]} : (app t1 t2)[σ,] = app t1[σ,] t2[σ,] := by
   simp [SubstMap.smap]
 
 @[simp]
-theorem Term.smap_lam {A t} {σ : SubstVec [Term, Ty]}
+theorem Term.smap_term_ty_lam {A t} {σ : SubstVec [Term, Ty]}
   : (lam A t)[σ,] = lam A[σ.get Ty 1] t[σ.lift [1, 0],]
 := by simp [SubstMap.smap]
 
 @[simp]
-theorem Term.smap_tapp {t1 t2} {σ : SubstVec [Term, Ty]}
+theorem Term.smap_term_ty_tapp {t1 t2} {σ : SubstVec [Term, Ty]}
   : (tapp t1 t2)[σ,] = tapp t1[σ,] t2[σ.get Ty 1]
 := by simp [SubstMap.smap]
 
 @[simp]
-theorem Term.smap_tlam {t} {σ : SubstVec [Term, Ty]}
+theorem Term.smap_term_ty_tlam {t} {σ : SubstVec [Term, Ty]}
   : (tlam t)[σ,] = tlam t[σ.map 𝐭[λ (τ : Subst Term) => τ⟨Ren.add Ty 1⟩, .lift],]
 := by simp [SubstMap.smap]
 
 @[simp]
-theorem Term.smap_zero {σ : SubstVec [Term, Ty]} : zero[σ,] = zero := by
+theorem Term.smap_term_ty_zero {σ : SubstVec [Term, Ty]} : zero[σ,] = zero := by
   simp [SubstMap.smap]
 
 @[simp]
-theorem Term.smap_succ {t} {σ : SubstVec [Term, Ty]} : (succ t)[σ,] = succ t[σ,] := by
+theorem Term.smap_term_ty_succ {t} {σ : SubstVec [Term, Ty]} : (succ t)[σ,] = succ t[σ,] := by
   simp [SubstMap.smap]
 
 @[simp]
-theorem Term.smap_nrec {m z s n} {σ : SubstVec [Term, Ty]}
+theorem Term.smap_term_ty_nrec {m z s n} {σ : SubstVec [Term, Ty]}
   : (nrec m z s n)[σ,] = nrec m[σ.get Ty 1] z[σ,] s[σ.lift [2, 0],] n[σ,]
 := by simp [SubstMap.smap]
 
 @[simp]
-theorem Subst.test2 {T V} [RenMap T V] (r : RenVec V) : (Subst.id T)⟨r,⟩ = Subst.id T := sorry
+instance : SubstMap Term [Term] where
+  smap σ := Term.smap (σ.get Term 0, Subst.id Ty, .unit)
+
+@[simp]
+theorem Term.smap_term_var {x} {σ : SubstVec [Term]} : (var x)[σ,] = (σ.get Term 0).act x := by
+  simp [SubstMap.smap]
+
+@[simp]
+theorem Term.smap_term_app {t1 t2} {σ : SubstVec [Term]} : (app t1 t2)[σ,] = app t1[σ,] t2[σ,] := by
+  simp [SubstMap.smap]
+
+@[simp]
+theorem Term.smap_term_lam {A t} {σ : SubstVec [Term]}
+  : (lam A t)[σ,] = lam A t[σ.lift [1],]
+:= by simp [SubstMap.smap]; sorry
+
+@[simp]
+theorem Term.smap_term_tapp {t1 t2} {σ : SubstVec [Term]}
+  : (tapp t1 t2)[σ,] = tapp t1[σ,] t2
+:= by simp [SubstMap.smap]; sorry
+
+@[simp]
+theorem Term.smap_term_tlam {t} {σ : SubstVec [Term]}
+  : (tlam t)[σ,] = tlam t[σ.map 𝐭[λ (τ : Subst Term) => τ⟨Ren.add Ty 1⟩],]
+:= by simp [SubstMap.smap]; sorry
+
+@[simp]
+theorem Term.smap_term_zero {σ : SubstVec [Term]} : zero[σ,] = zero := by
+  simp [SubstMap.smap]
+
+@[simp]
+theorem Term.smap_term_succ {t} {σ : SubstVec [Term]} : (succ t)[σ,] = succ t[σ,] := by
+  simp [SubstMap.smap]
+
+@[simp]
+theorem Term.smap_term_nrec {m z s n} {σ : SubstVec [Term]}
+  : (nrec m z s n)[σ,] = nrec m z[σ,] s[σ.lift [2],] n[σ,]
+:= by simp [SubstMap.smap]; sorry
+
+@[simp]
+instance : SubstMap Term [Ty] where
+  smap σ := Term.smap (Subst.id Term, σ.get Ty 0, .unit)
+
+@[simp]
+theorem Term.smap_ty_var {x} {σ : SubstVec [Ty]} : (var x)[σ,] = var x := by
+  simp [SubstMap.smap]
+
+@[simp]
+theorem Term.smap_ty_app {t1 t2} {σ : SubstVec [Ty]} : (app t1 t2)[σ,] = app t1[σ,] t2[σ,] := by
+  simp [SubstMap.smap]
+
+@[simp]
+theorem Term.smap_ty_lam {A t} {σ : SubstVec [Ty]}
+  : (lam A t)[σ,] = lam A[σ.get Ty 0] t[σ,]
+:= by simp [SubstMap.smap]
+
+@[simp]
+theorem Term.smap_ty_tapp {t1 t2} {σ : SubstVec [Ty]}
+  : (tapp t1 t2)[σ,] = tapp t1[σ,] t2[σ.get Ty 0]
+:= by simp [SubstMap.smap]
+
+@[simp]
+theorem Term.smap_ty_tlam {t} {σ : SubstVec [Ty]}
+  : (tlam t)[σ,] = tlam t[σ.map 𝐭[.lift],]
+:= by simp [SubstMap.smap]; sorry
+
+@[simp]
+theorem Term.smap_ty_zero {σ : SubstVec [Ty]} : zero[σ,] = zero := by
+  simp [SubstMap.smap]
+
+@[simp]
+theorem Term.smap_ty_succ {t} {σ : SubstVec [Ty]} : (succ t)[σ,] = succ t[σ,] := by
+  simp [SubstMap.smap]
+
+@[simp]
+theorem Term.smap_ty_nrec {m z s n} {σ : SubstVec [Ty]}
+  : (nrec m z s n)[σ,] = nrec m[σ.get Ty 0] z[σ,] s[σ,] n[σ,]
+:= by simp [SubstMap.smap]
+
+@[reducible, simp]
+instance instSubstMapAll_Term : SubstMapAll [Term] := .cons .nil
+
+@[reducible, simp]
+instance instSubstMapAll_Term_Ty : SubstMapAll [Term, Ty] := .cons instSubstMapAll_Ty
 
 @[simp]
 theorem Term.from_action_smap {t : Action Term} {σ : SubstVec [Term]}
@@ -343,20 +496,12 @@ instance : SubstMapRenComposeLeft Term [Term, Ty] where
 instance : SubstMapRenComposeRight Term [Term, Ty] where
   apply_ren_compose_right := by sorry
 
+@[grind =]
 theorem Term.smap_composition_lemma {s : Term} {σ : Subst Term} {τ : Subst Ty} :
   s[σ, τ] = s[τ][σ]
 := by
   induction s generalizing σ τ
-  case var => sorry
-  case app =>
-    simp +instances [*]
-  case lam => sorry
-  case tapp => sorry
-  case tlam => sorry
-  case zero => sorry
-  case succ => sorry
-  case nrec =>
-    sorry
+  all_goals try solve | simp [*]
 
 @[simp]
 theorem Term.apply_compose
@@ -377,35 +522,37 @@ theorem Term.apply_compose
   case nrec => sorry
   case tapp => sorry
   case var =>
-    rcases σ with ⟨σ1, σ2, u1⟩
-    rcases τ with ⟨τ1, τ2, u2⟩
-    cases u1; cases u2; case _ x =>
-    simp; generalize zdef : σ1.act x = z
-    cases z <;> simp
-    case re y =>
-      unfold SubstMap.smap
-      unfold instSubstMapActionConsNil; simp
-      unfold instSubstMapSubst; simp
-      unfold Subst.smap; simp
-      rw [zdef]; unfold LeanSubst.smap
-      unfold instSubstMapAction; simp
-    case su t =>
-      unfold SubstMap.smap
-      unfold instSubstMapActionConsNil; simp
-      unfold instSubstMapSubst; simp
-      unfold Subst.smap; simp
-      rw [zdef]; unfold LeanSubst.smap
-      unfold instSubstMapAction; simp
-      unfold instSubstMapAllConsTermTyNil
-      unfold SubstMapAll.get; simp
-      unfold instSubstMap_Term_Term; simp
-      have lem := Term.smap_composition_lemma (s := t) (σ := τ1) (τ := τ2)
-      unfold LeanSubst.smap at lem
-      unfold instSubstMapTermConsTyNil at lem
-      unfold instSubstMap_Term_Term at lem; simp at lem
-      rw [lem]
-      unfold instSubstMap_Term_Ty; simp
-      congr
+    sorry
+    -- rcases σ with ⟨σ1, σ2, u1⟩
+    -- rcases τ with ⟨τ1, τ2, u2⟩
+    -- cases u1; cases u2; case _ x =>
+    -- simp
+    -- simp; generalize zdef : σ1.act x = z
+    -- cases z <;> simp
+    -- case re y =>
+    --   unfold SubstMap.smap
+    --   unfold instSubstMapActionConsNil; simp
+    --   unfold instSubstMapSubst; simp
+    --   unfold Subst.smap; simp
+    --   rw [zdef]; unfold LeanSubst.smap
+    --   unfold instSubstMapAction; simp
+
+      -- unfold SubstMap.smap
+      -- unfold instSubstMapActionConsNil; simp
+      -- unfold instSubstMapSubst; simp
+      -- unfold Subst.smap; simp
+      -- rw [zdef]; unfold LeanSubst.smap
+      -- unfold instSubstMapAction; simp
+      -- unfold instSubstMapAllConsTermTyNil
+      -- unfold SubstMapAll.get; simp
+      -- unfold instSubstMap_Term_Term; simp
+      -- have lem := Term.smap_composition_lemma (s := t) (σ := τ1) (τ := τ2)
+      -- unfold LeanSubst.smap at lem
+      -- unfold instSubstMapTermConsTyNil at lem
+      -- unfold instSubstMap_Term_Term at lem; simp at lem
+      -- rw [lem]
+      -- unfold instSubstMap_Term_Ty; simp
+      -- congr
 
 instance : SubstMapCompose Term [Term, Ty] where
   apply_compose := by intro s σ τ; simp [SubstMap.smap]; try rfl
